νDgnSet: work in progress on degeneracies in all directions

theories/νSet/νDgnSet.v
@@ -15,72 +15,13 @@ Module νDgnSet (A: νSet.AritySig).
 Import A.
 
 Module Import νSet := νSet.νSet A.
+Arguments mkDepsRestr {p k} depsCohs.
 
 Definition FramePrev {p k} (deps: DepsRestr p.+1 k): Type :=
   deps.(_frames).2.
 
 Definition FrameBase {p k} (deps: DepsRestr p.+1 k): Type :=
   mkFrame (deps.(1)).
-
-Definition NextDepsRestr {p k} (depsCohs: DepsCohs p k): DepsRestr p.+1 k :=
-  mkDepsRestr.
-
-Fixpoint mkReflFrameTypes {p k}: DepsRestr p k -> Type :=
-  match p with
-  | 0 => fun _ => unit
-  | p'.+1 => fun deps =>
-    { R: mkReflFrameTypes deps.(1) &T
-          FramePrev deps -> FrameBase deps }
-  end.
-
-Class DepsReflRestr p k := {
-  _deps: DepsRestr p k;
-  _reflFrames: mkReflFrameTypes _deps;
-}.
-
-#[local]
-Instance proj1DepsRefl {p k}
-  `(deps: DepsReflRestr p.+1 k): DepsReflRestr p k.+1 :=
-{|
-  _deps := proj1DepsRestr (deps.(_deps));
-  _reflFrames := deps.(_reflFrames).1;
-|}.
-
-Declare Scope depsreflrestr_scope.
-Delimit Scope depsreflrestr_scope with depsreflrestr.
-Bind Scope depsreflrestr_scope with DepsReflRestr.
-Notation "x .(1)" := (proj1DepsRefl x%_depsreflrestr)
-  (at level 1, left associativity, format "x .(1)"): depsreflrestr_scope.
-
-
-Definition ReflFramePrev {p k} (deps: DepsReflRestr p.+1 k): Type :=
-  FramePrev deps.(_deps).
-
-Definition ReflFrameBase {p k} (deps: DepsReflRestr p.+1 k): Type :=
-  FrameBase deps.(_deps).
-
-Definition restrFrame {p k} i (Hi: i <= k) (deps: DepsRestr p.+1 k) (ε: arity):
-  FrameBase deps -> FramePrev deps :=
-  deps.(_restrFrames).2 i Hi ε.
-
-Definition reflFrame {p k} (deps: DepsReflRestr p.+1 k):
-  ReflFramePrev deps -> ReflFrameBase deps :=
-  deps.(_reflFrames).2.
-
-Definition mkIdReflRestrFrameType {p k}
-  (deps: DepsReflRestr p.+1 k): Type :=
-  forall ε (d: ReflFramePrev deps),
-  restrFrame k leR_refl deps.(_deps) ε (reflFrame deps d) = d.
-
-Fixpoint mkIdReflRestrFrameTypes {p}:
-  forall {k} (deps: DepsReflRestr p k), Type :=
-  match p with
-  | 0 => fun _ _ => unit
-  | S p =>
-    fun k deps =>
-    { _: mkIdReflRestrFrameTypes deps.(1) &T
-      mkIdReflRestrFrameType deps }
-  end.
 
 Definition PaintingPrev {p k} (deps: DepsRestr p.+1 k):
   FramePrev deps -> Type :=
@@ -90,154 +31,203 @@ Definition PaintingBase {p k} (deps: DepsRestr p.+1 k)
   (extraDeps: DepsRestrExtension p.+1 k deps): FrameBase deps -> Type :=
   (mkPaintings (deps; extraDeps)).2.
 
-Definition ReflPaintingPrev {p k} (deps: DepsReflRestr p.+1 k):
-  ReflFramePrev deps -> Type :=
-  PaintingPrev deps.(_deps).
+Fixpoint mkReflFrameBelowTypes {p k}: DepsRestr p k -> Type :=
+  match p with
+  | 0 => fun _ => unit
+  | p'.+1 => fun deps =>
+    { R: mkReflFrameBelowTypes deps.(1) &T
+          forall i (Hi: i <= k), FramePrev deps -> FrameBase deps }
+  end.
 
-Definition ReflPaintingBase {p k} (deps: DepsReflRestr p.+1 k)
-  (extraDeps: DepsRestrExtension p.+1 k deps.(_deps)):
-  ReflFrameBase deps -> Type :=
-  PaintingBase deps.(_deps) extraDeps.
+Fixpoint mkReflFrameAboveTypes {p k}: DepsRestr p k -> Type :=
+  match p with
+  | 0 => fun _ => unit
+  | p'.+1 => fun deps =>
+    { R: mkReflFrameAboveTypes deps.(1) &T
+          forall i (Hi: i <= p') (d: FramePrev deps), PaintingPrev deps d -> mkFrame deps }
+  end.
 
-Definition mkReflPaintingType {p k} (deps: DepsReflRestr p.+1 k)
-  `(extraDeps: DepsRestrExtension p.+1 k deps.(_deps)) :=
-  forall (d: ReflFramePrev deps),
-  ReflPaintingPrev deps d ->
-  ReflPaintingBase deps extraDeps (reflFrame deps d).
+Class DepsReflBelow p k := {
+  _depsRestr: DepsRestr p k;
+  _reflFramesBelow: mkReflFrameBelowTypes _depsRestr;
+}.
 
-Fixpoint mkReflPaintingTypes {p}:
-  forall {k} (deps: DepsReflRestr p k)
-  `(extraDeps: DepsRestrExtension p k deps.(_deps)), Type :=
+#[local]
+Instance proj1DepsReflBelow {p k}
+  (deps: DepsReflBelow p.+1 k): DepsReflBelow p k.+1 :=
+{|
+  _depsRestr := proj1DepsRestr (deps.(_depsRestr));
+  _reflFramesBelow := deps.(_reflFramesBelow).1;
+|}.
+
+Declare Scope depsreflbelow_scope.
+Delimit Scope depsreflbelow_scope with depsreflbelow.
+Bind Scope depsreflbelow_scope with DepsReflBelow.
+Notation "x .(1)" := (proj1DepsReflBelow x%depsreflbelow)
+  (at level 1, left associativity, format "x .(1)"): depsreflbelow_scope.
+
+Definition mkIdReflRestrFrameBelowType {p k}
+  (deps: DepsReflBelow p.+1 k): Type :=
+  forall i (Hi: i <= k) ε (d: FramePrev deps.(_depsRestr)),
+  deps.(_depsRestr).(_restrFrames).2 i Hi ε (deps.(_reflFramesBelow).2 i Hi d) = d.
+
+Fixpoint mkIdReflRestrFrameBelowTypes {p}:
+  forall {k} (deps: DepsReflBelow p k), Type :=
+  match p with
+  | 0 => fun _ _ => unit
+  | S p =>
+    fun k deps =>
+    { _: mkIdReflRestrFrameBelowTypes deps.(1) &T
+      mkIdReflRestrFrameBelowType deps }
+  end.
+
+Definition mkReflPaintingBelowType {p k} (deps: DepsReflBelow p.+1 k)
+  (extraDeps: DepsRestrExtension p.+1 k deps.(_depsRestr)) :=
+  forall i (Hi: i <= k) (d: FramePrev deps.(_depsRestr)),
+  PaintingPrev deps.(_depsRestr) d ->
+  PaintingBase deps.(_depsRestr) extraDeps (deps.(_reflFramesBelow).2 i Hi d).
+
+Fixpoint mkReflPaintingBelowTypes {p}:
+  forall {k} (deps: DepsReflBelow p k)
+  (extraDeps: DepsRestrExtension p k deps.(_depsRestr)), Type :=
   match p with
   | 0 => fun _ _ _ => unit
   | S p =>
     fun k deps extraDeps =>
-    { _: mkReflPaintingTypes deps.(1) (deps.(_deps); extraDeps) &T
-      mkReflPaintingType deps extraDeps }
+    { _: mkReflPaintingBelowTypes deps.(1) (deps.(_depsRestr); extraDeps) &T
+      mkReflPaintingBelowType deps extraDeps }
   end.
 
-Class CohReflRestrFrameTypeBlock {p k} (deps: DepsRestr p k) := {
-  CohReflRestrFrameTypesDef: Type;
-  ReflFramesDef: CohReflRestrFrameTypesDef -> mkReflFrameTypes deps;
+Class CohReflRestrFrameBelowInfTypeBlock {p k} (deps: DepsRestr p k) := {
+  CohReflRestrFrameBelowInfTypesDef: Type;
+  ReflFramesBelowDef: CohReflRestrFrameBelowInfTypesDef -> mkReflFrameBelowTypes deps;
 }.
 
 #[local]
-Instance toDepsRefl {p k}
+Instance toDepsReflBelow {p k}
   (depsCohs: DepsCohs p k)
-  (reflFrames: mkReflFrameTypes depsCohs.(νSet._deps)): DepsReflRestr p k :=
-  {| _deps := depsCohs.(νSet._deps);
-     _reflFrames := reflFrames;
+  (reflFrames: mkReflFrameBelowTypes depsCohs.(_deps)): DepsReflBelow p k :=
+  {| _depsRestr := depsCohs.(_deps);
+     _reflFramesBelow := reflFrames;
   |}.
 
-Definition mkCohReflRestrFrameTypesStep {p k} (deps: DepsCohs p.+1 k)
-  (reflFrames: mkReflFrameTypes deps.(νSet._deps))
-  (prev: CohReflRestrFrameTypeBlock (NextDepsRestr deps.(1))): Type :=
-  { Q: prev.(CohReflRestrFrameTypesDef) &T
-    forall i (Hi: i <= k) (ε: arity) (d: ReflFrameBase (toDepsRefl deps reflFrames)),
-    let reflFrame': FramePrev _ -> FrameBase _ := (prev.(ReflFramesDef) Q).2 in
-    reflFrame _ (restrFrame i Hi _ ε d) =
-    restrFrame i (↑ Hi) _ ε (reflFrame' d) }.
+Definition mkCohReflRestrFrameBelowInfTypesStep {p k} (deps: DepsCohs p.+1 k)
+  (reflFramesBelow: mkReflFrameBelowTypes deps.(_deps))
+  (prev: CohReflRestrFrameBelowInfTypeBlock (mkDepsRestr deps.(1))): Type :=
+  { Q: prev.(CohReflRestrFrameBelowInfTypesDef) &T
+    forall q r (Hq: q <= k) (Hr: r <= q) (ε: arity) (d: FrameBase deps.(_deps)),
+    reflFramesBelow.2 q Hq (deps.(_deps).(_restrFrames).2 r (Hr ↕ Hq) ε d) =
+    mkRestrFrame r (Hr ↕ ↑ Hq) ε ((prev.(ReflFramesBelowDef) Q).2 q.+1 (⇑ Hq) d) }.
 
-Definition mkReflLayer {p k} (deps: DepsCohs p.+1 k)
-  (reflFrames: mkReflFrameTypes deps.(νSet._deps))
-  (reflPaintings: mkReflPaintingTypes (toDepsRefl deps reflFrames)
+Definition mkReflLayerBelow {p k} (deps: DepsCohs p.+1 k)
+  (reflFramesBelow: mkReflFrameBelowTypes deps.(_deps))
+  (reflPaintingsBelow: mkReflPaintingBelowTypes (toDepsReflBelow deps reflFramesBelow)
     deps.(_extraDeps))
-  (prev: CohReflRestrFrameTypeBlock (NextDepsRestr deps.(1)))
-  (cohFrames: mkCohReflRestrFrameTypesStep deps reflFrames prev)
-  (d: ReflFrameBase (toDepsRefl deps reflFrames)):
-  mkLayer deps.(νSet._deps).(_restrFrames) d ->
+  (prev: CohReflRestrFrameBelowInfTypeBlock (mkDepsRestr deps.(1)))
+  (cohFrames: mkCohReflRestrFrameBelowInfTypesStep deps reflFramesBelow prev)
+  i (Hi: i <= k)
+  (d: FrameBase deps.(_deps)):
+  mkLayer deps.(_deps).(_restrFrames) d ->
   mkLayer
-    (NextDepsRestr deps.(1)).(_restrFrames)
-    ((prev.(ReflFramesDef) cohFrames.1).2 d) :=
+    (mkDepsRestr deps.(1)).(_restrFrames)
+    ((prev.(ReflFramesBelowDef) cohFrames.1).2 i.+1 (⇑ Hi) d) :=
   fun l ε =>
-    rew [(NextDepsRestr deps.(1)).(_paintings).2] cohFrames.2 0 leR_O ε d in
-    reflPaintings.2 (restrFrame 0 leR_O (toDepsRefl deps reflFrames).(_deps)
-      ε d) (l ε).
+    rew [(mkDepsRestr deps.(1)).(_paintings).2]
+      cohFrames.2 i 0 Hi leR_O ε d in
+    reflPaintingsBelow.2 i Hi (deps.(_deps).(_restrFrames).2 0 leR_O ε d) (l ε).
 
-Fixpoint mkCohReflRestrFrameTypesAndReflFrames {p k}:
-  forall (deps: DepsCohs p k) (reflFrames: mkReflFrameTypes deps.(νSet._deps))
-    (reflPaintings: mkReflPaintingTypes (toDepsRefl deps reflFrames)
+Fixpoint mkCohReflRestrFrameBelowInfTypesAndReflFramesBelow {p k}:
+  forall (deps: DepsCohs p k) (reflFramesBelow: mkReflFrameBelowTypes deps.(_deps))
+    (reflPaintingsBelow: mkReflPaintingBelowTypes (toDepsReflBelow deps reflFramesBelow)
       deps.(_extraDeps)),
-    CohReflRestrFrameTypeBlock (NextDepsRestr deps) :=
+    CohReflRestrFrameBelowInfTypeBlock (mkDepsRestr deps) :=
   match p with
   | 0 =>
     fun deps reflFrames reflPaintings =>
     {|
-      CohReflRestrFrameTypesDef := unit;
-      ReflFramesDef _ := (tt; fun _ => tt):
-        mkReflFrameTypes (NextDepsRestr deps)
+      CohReflRestrFrameBelowInfTypesDef := unit;
+      ReflFramesBelowDef _ :=
+        let reflFrame0: forall i (Hi: i <= k),
+          FramePrev (mkDepsRestr deps) -> FrameBase (mkDepsRestr deps) :=
+          fun _ _ d => d in
+        (((tt: mkReflFrameBelowTypes (mkDepsRestr deps).(1)); reflFrame0):
+          mkReflFrameBelowTypes (mkDepsRestr deps))
     |}
   | S p =>
-    fun deps reflFrames reflPaintings =>
-    let prev := mkCohReflRestrFrameTypesAndReflFrames deps.(1)
-      reflFrames.1 reflPaintings.1 in
+    fun deps reflFramesBelow reflPaintingsBelow =>
+    let prev := mkCohReflRestrFrameBelowInfTypesAndReflFramesBelow deps.(1)
+      reflFramesBelow.1 reflPaintingsBelow.1 in
     {|
-      CohReflRestrFrameTypesDef := mkCohReflRestrFrameTypesStep deps
-        reflFrames prev;
-      ReflFramesDef Q :=
-        let prevFrames := prev.(ReflFramesDef) Q.1 in
-        let reflFrame d := (prevFrames.2 d.1;
-          mkReflLayer deps reflFrames reflPaintings prev Q d.1 d.2) in
-        (prevFrames; reflFrame): mkReflFrameTypes (NextDepsRestr deps)
+      CohReflRestrFrameBelowInfTypesDef := mkCohReflRestrFrameBelowInfTypesStep deps
+        reflFramesBelow prev;
+      ReflFramesBelowDef Q :=
+        let prevFrames := prev.(ReflFramesBelowDef) Q.1 in
+        let reflFrame i (Hi: i <= k) d := (prevFrames.2 i.+1 (⇑ Hi) d.1;
+          mkReflLayerBelow deps reflFramesBelow reflPaintingsBelow prev Q i Hi d.1 d.2) in
+        (prevFrames; reflFrame): mkReflFrameBelowTypes (mkDepsRestr deps)
     |}
   end.
 
-Definition mkCohReflRestrFrameTypes {p k}
+Definition mkCohReflRestrFrameBelowInfTypes {p k}
   (deps: DepsCohs p k)
-  (reflFrames: mkReflFrameTypes deps.(νSet._deps))
-  (reflPaintings: mkReflPaintingTypes (toDepsRefl deps reflFrames)
+  (reflFramesBelow: mkReflFrameBelowTypes deps.(_deps))
+  (reflPaintingsBelow: mkReflPaintingBelowTypes (toDepsReflBelow deps reflFramesBelow)
     deps.(_extraDeps)): Type :=
-  (mkCohReflRestrFrameTypesAndReflFrames deps reflFrames
-    reflPaintings).(CohReflRestrFrameTypesDef).
+  (mkCohReflRestrFrameBelowInfTypesAndReflFramesBelow deps reflFramesBelow
+    reflPaintingsBelow).(CohReflRestrFrameBelowInfTypesDef).
 
-Definition mkIdReflRestrPaintingType {p k}
+Definition mkIdReflRestrPaintingBelowType {p k}
   (deps: DepsCohs p.+1 k)
-  (reflFrames: mkReflFrameTypes deps.(νSet._deps))
-  (reflPaintings: mkReflPaintingTypes (toDepsRefl deps reflFrames)
+  (reflFramesBelow: mkReflFrameBelowTypes deps.(_deps))
+  (reflPaintingsBelow: mkReflPaintingBelowTypes (toDepsReflBelow deps reflFramesBelow)
     deps.(_extraDeps))
-  (idReflRestrFrames: mkIdReflRestrFrameTypes (toDepsRefl deps reflFrames)):
+  (idReflRestrFrames: mkIdReflRestrFrameBelowTypes (toDepsReflBelow deps reflFramesBelow)):
   Type :=
-  forall (ε: arity) (d: ReflFramePrev (toDepsRefl deps reflFrames))
-    (c: ReflPaintingPrev (toDepsRefl deps reflFrames) d),
-  rew [ReflPaintingPrev (toDepsRefl deps reflFrames)] idReflRestrFrames.2 ε d in
-  deps.(_restrPaintings).2 k leR_refl ε (reflFrames.2 d) (reflPaintings.2 d c) = c.
+  forall i (Hi: i <= k) (ε: arity)
+    (d: FramePrev deps.(_deps))
+    (c: PaintingPrev deps.(_deps) d),
+  rew [PaintingPrev deps.(_deps)] idReflRestrFrames.2 i Hi ε d in
+  deps.(_restrPaintings).2 i Hi ε
+    (reflFramesBelow.2 i Hi d) (reflPaintingsBelow.2 i Hi d c) = c.
 
-Fixpoint mkIdReflRestrPaintingTypes {p}:
+Fixpoint mkIdReflRestrPaintingBelowTypes {p}:
   forall {k} (deps: DepsCohs p k)
-    (reflFrames: mkReflFrameTypes deps.(νSet._deps))
-    (reflPaintings: mkReflPaintingTypes (toDepsRefl deps reflFrames)
+    (reflFramesBelow: mkReflFrameBelowTypes deps.(_deps))
+    (reflPaintingsBelow: mkReflPaintingBelowTypes (toDepsReflBelow deps reflFramesBelow)
       deps.(_extraDeps))
-    (idReflRestrFrames: mkIdReflRestrFrameTypes (toDepsRefl deps reflFrames)),
+    (idReflRestrFrames: mkIdReflRestrFrameBelowTypes (toDepsReflBelow deps reflFramesBelow)),
   Type :=
   match p with
   | 0 => fun _ _ _ _ _ => unit
   | S p =>
-    fun k deps reflFrames reflPaintings idReflRestrFrames =>
-    { _: mkIdReflRestrPaintingTypes deps.(1) reflFrames.1 reflPaintings.1 idReflRestrFrames.1 &T
-      mkIdReflRestrPaintingType deps reflFrames reflPaintings
+    fun k deps reflFramesBelow reflPaintingsBelow idReflRestrFrames =>
+    { _: mkIdReflRestrPaintingBelowTypes deps.(1) reflFramesBelow.1 reflPaintingsBelow.1 idReflRestrFrames.1 &T
+      mkIdReflRestrPaintingBelowType deps reflFramesBelow reflPaintingsBelow
         idReflRestrFrames }
   end.
 
 Class DepsReflCohs p k := {
   _depsCohs2: DepsCohs2 p k;
-  _reflFrameDeps: mkReflFrameTypes _depsCohs.(νSet._deps);
-  _reflPaintingDeps: mkReflPaintingTypes
-    (toDepsRefl _depsCohs _reflFrameDeps) _depsCohs.(_extraDeps);
-  _idReflRestrFrames: mkIdReflRestrFrameTypes
-    (toDepsRefl _depsCohs _reflFrameDeps);
-  _idReflRestrPaintings: mkIdReflRestrPaintingTypes _depsCohs _reflFrameDeps _reflPaintingDeps _idReflRestrFrames;
-  _cohReflRestrFrames: mkCohReflRestrFrameTypes _depsCohs _reflFrameDeps _reflPaintingDeps
+  _reflFramesBelow': mkReflFrameBelowTypes _depsCohs.(_deps);
+  _reflFramesAbove: mkReflFrameAboveTypes _depsCohs.(_deps);
+  _reflPaintingsBelow: mkReflPaintingBelowTypes
+    (toDepsReflBelow _depsCohs _reflFramesBelow') _depsCohs.(_extraDeps);
+  _idReflRestrFramesBelow: mkIdReflRestrFrameBelowTypes
+    (toDepsReflBelow _depsCohs _reflFramesBelow');
+  _idReflRestrPaintingsBelow: mkIdReflRestrPaintingBelowTypes _depsCohs _reflFramesBelow' _reflPaintingsBelow _idReflRestrFramesBelow;
+  _cohReflRestrFramesBelowInf: mkCohReflRestrFrameBelowInfTypes _depsCohs _reflFramesBelow' _reflPaintingsBelow
 }.
 
 #[local]
-Instance proj1DepsReflCohs {p k} `(depsCohs: DepsReflCohs p.+1 k): DepsReflCohs p k.+1 :=
+Instance proj1DepsReflCohs {p k} (depsCohs: DepsReflCohs p.+1 k): DepsReflCohs p k.+1 :=
 {|
   _depsCohs2 := (depsCohs.(_depsCohs2)).(1);
-  _reflFrameDeps := depsCohs.(_reflFrameDeps).1;
-  _reflPaintingDeps := depsCohs.(_reflPaintingDeps).1;
-  _idReflRestrFrames := depsCohs.(_idReflRestrFrames).1;
-  _idReflRestrPaintings := depsCohs.(_idReflRestrPaintings).1;
-  _cohReflRestrFrames := depsCohs.(_cohReflRestrFrames).1;
+  _reflFramesBelow' := depsCohs.(_reflFramesBelow').1;
+  _reflFramesAbove := depsCohs.(_reflFramesAbove).1;
+  _reflPaintingsBelow := depsCohs.(_reflPaintingsBelow).1;
+  _idReflRestrFramesBelow := depsCohs.(_idReflRestrFramesBelow).1;
+  _idReflRestrPaintingsBelow := depsCohs.(_idReflRestrPaintingsBelow).1;
+  _cohReflRestrFramesBelowInf := depsCohs.(_cohReflRestrFramesBelowInf).1;
 |}.
 
 Declare Scope depsreflcohs_scope.
@@ -246,189 +236,422 @@ Bind Scope depsreflcohs_scope with DepsReflCohs.
 Notation "x .(1)" := (proj1DepsReflCohs x%_depsreflcohs)
   (at level 1, left associativity, format "x .(1)"): depsreflcohs_scope.
 
-Definition ReflOfReflCohs {p k}
-  `(depsCohs: DepsReflCohs p k): DepsReflRestr p k :=
+Definition ReflBelowOfReflCohs {p k}
+  (depsCohs: DepsReflCohs p k): DepsReflBelow p k :=
 {|
-  _deps := depsCohs.(_depsCohs2).(_depsCohs).(νSet._deps);
-  _reflFrames := depsCohs.(_reflFrameDeps);
+  _depsRestr := depsCohs.(_depsCohs2).(_depsCohs).(_deps);
+  _reflFramesBelow := depsCohs.(_reflFramesBelow');
 |}.
 
 Definition RestrOfReflCohs {p k}
-  `(depsCohs: DepsReflCohs p k): DepsRestr p k :=
-  (ReflOfReflCohs depsCohs).(_deps).
+  (depsCohs: DepsReflCohs p k): DepsRestr p k :=
+  (ReflBelowOfReflCohs depsCohs).(_depsRestr).
 
 Definition CohsOfReflCohs {p k}
-  `(depsCohs: DepsReflCohs p k): DepsCohs p k :=
+  (depsCohs: DepsReflCohs p k): DepsCohs p k :=
   depsCohs.(_depsCohs2).(_depsCohs).
 
 Definition RestrExtOfReflCohs {p k}
-  `(depsCohs: DepsReflCohs p k): DepsRestrExtension p k
+  (depsCohs: DepsReflCohs p k): DepsRestrExtension p k
     (RestrOfReflCohs depsCohs) :=
   depsCohs.(_depsCohs2).(_depsCohs).(_extraDeps).
 
 Definition CohsExtOfReflCohs {p k}
-  `(depsCohs: DepsReflCohs p k): DepsCohsExtension p k
+  (depsCohs: DepsReflCohs p k): DepsCohsExtension p k
     (CohsOfReflCohs depsCohs) :=
   depsCohs.(_depsCohs2).(_extraDepsCohs).
 
-Definition mkReflFrames {p k} (deps: DepsReflCohs p k):
-  mkReflFrameTypes (NextDepsRestr (CohsOfReflCohs deps)) :=
-  (mkCohReflRestrFrameTypesAndReflFrames
+Definition mkReflFramesBelow {p k} (deps: DepsReflCohs p k):
+  mkReflFrameBelowTypes (mkDepsRestr (CohsOfReflCohs deps)) :=
+  (mkCohReflRestrFrameBelowInfTypesAndReflFramesBelow
     deps.(_depsCohs2).(_depsCohs)
-    deps.(_reflFrameDeps)
-    deps.(_reflPaintingDeps)).(ReflFramesDef) deps.(_cohReflRestrFrames).
+    deps.(_reflFramesBelow')
+    deps.(_reflPaintingsBelow)).(ReflFramesBelowDef) deps.(_cohReflRestrFramesBelowInf).
 
-Definition mkReflFrame {p k} (deps: DepsReflCohs p.+1 k):
-  FramePrev (NextDepsRestr (CohsOfReflCohs deps)) ->
-  FrameBase (NextDepsRestr (CohsOfReflCohs deps)) :=
-  (mkReflFrames deps).2.
+Definition mkReflFrameBelow {p k} (deps: DepsReflCohs p k):
+  forall i (Hi: i <= k),
+  FramePrev (mkDepsRestr (CohsOfReflCohs deps)) ->
+  FrameBase (mkDepsRestr (CohsOfReflCohs deps)) :=
+  (mkReflFramesBelow deps).2.
 
-Definition NextDepsRefl {p k} (deps: DepsReflCohs p k): DepsReflRestr p.+1 k :=
-  {| _deps := NextDepsRestr (CohsOfReflCohs deps);
-     _reflFrames := mkReflFrames deps
+Definition mkDepsReflBelow {p k} (deps: DepsReflCohs p k): DepsReflBelow p.+1 k :=
+  {| _depsRestr := mkDepsRestr (CohsOfReflCohs deps);
+     _reflFramesBelow := mkReflFramesBelow deps
   |}.
 
-Definition restrPainting {p k} (deps: DepsReflCohs p.+1 k):
-  forall i (Hi: i <= k) (ε: arity) (d: ReflFrameBase (ReflOfReflCohs deps)),
-  ReflPaintingBase (ReflOfReflCohs deps) (RestrExtOfReflCohs deps) d ->
-  ReflPaintingPrev (ReflOfReflCohs deps)
-    (restrFrame i Hi (RestrOfReflCohs deps) ε d) :=
-  deps.(_depsCohs2).(_depsCohs).(_restrPaintings).2.
+Definition mkCohReflRestrFrameBelowSupType {p k}
+  (deps: DepsReflCohs p.+1 k): Type :=
+  forall q r (Hq: q <= r) (Hr: r <= k) (ε: arity) (d: FrameBase (RestrOfReflCohs deps)),
+  deps.(_reflFramesBelow').2 q (Hq ↕ Hr) ((RestrOfReflCohs deps).(_restrFrames).2 r Hr ε d) =
+  mkRestrFrame r.+1 (⇑ Hr) ε (mkReflFrameBelow deps.(1) q (Hq ↕ ↑ Hr) d).
 
-Definition reflPainting {p k} (deps: DepsReflCohs p.+1 k):
-  forall (d: ReflFramePrev (ReflOfReflCohs deps)),
-  ReflPaintingPrev (ReflOfReflCohs deps) d ->
-  ReflPaintingBase (ReflOfReflCohs deps) (RestrExtOfReflCohs deps)
-    (reflFrame (ReflOfReflCohs deps) d) :=
-  deps.(_reflPaintingDeps).2.
+Fixpoint mkCohReflRestrFrameBelowSupTypes {p}:
+  forall {k} (deps: DepsReflCohs p k), Type :=
+  match p with
+  | 0 => fun _ _ => unit
+  | S p =>
+    fun k deps =>
+    { _: mkCohReflRestrFrameBelowSupTypes deps.(1) &T
+      mkCohReflRestrFrameBelowSupType deps }
+  end.
 
-Definition mkIdReflRestrLayer {p k}
+Definition mkIdReflRestrLayerBelow {p k}
   (deps: DepsReflCohs p.+1 k)
+  i (Hi: i <= k)
   (ε: arity)
-  (d: ReflFrameBase (ReflOfReflCohs deps))
+  (d: FrameBase (RestrOfReflCohs deps))
   (l: mkLayer (RestrOfReflCohs deps).(_restrFrames) d)
-  (prevIdReflRestrFrames: mkIdReflRestrFrameTypes (NextDepsRefl deps.(1))):
-  rew [mkLayer _] prevIdReflRestrFrames.2 ε d in
+  (prevIdReflRestrFrames: mkIdReflRestrFrameBelowTypes (mkDepsReflBelow deps.(1))):
+  rew [mkLayer _] prevIdReflRestrFrames.2 i.+1 (⇑ Hi) ε d in
   mkRestrLayer deps.(_depsCohs2).(_depsCohs).(_restrPaintings)
-    (deps.(_depsCohs2).(_depsCohs).(_cohs)) k leR_refl ε _
-      (mkReflLayer deps.(_depsCohs2).(_depsCohs)
-        ((ReflOfReflCohs deps).(_reflFrames)) deps.(_reflPaintingDeps) _
-          deps.(_cohReflRestrFrames) d l) = l.
+    (deps.(_depsCohs2).(_depsCohs).(_cohs)) i Hi ε _
+      (mkReflLayerBelow deps.(_depsCohs2).(_depsCohs)
+        ((ReflBelowOfReflCohs deps).(_reflFramesBelow)) deps.(_reflPaintingsBelow) _
+          deps.(_cohReflRestrFramesBelowInf) i Hi d l) = l.
 Proof.
   apply functional_extensionality_dep.
   intros θ.
-  unfold mkRestrLayer, mkReflLayer.
-  rewrite <- (deps.(_idReflRestrPaintings).2 ε _ (l θ)).
+  unfold mkRestrLayer, mkReflLayerBelow.
+  rewrite <- (deps.(_idReflRestrPaintingsBelow).2 i Hi ε _ (l θ)).
   rewrite <- map_subst_app, <- map_subst.
-  unfold reflFrame, restrFrame, toDepsRefl, ReflPaintingPrev, PaintingPrev,
-         FramePrev, RestrOfReflCohs, mkFrame; simpl.
+  unfold toDepsReflBelow, PaintingPrev, FramePrev, RestrOfReflCohs, mkFrame; simpl.
   rewrite rew_map with
-    (P := fun x => deps.(_depsCohs2).(_depsCohs).(νSet._deps).(_paintings).2 x)
-    (f := fun x => (deps.(_depsCohs2).(_depsCohs).(νSet._deps).(_restrFrames).2 0 leR_O θ x)).
+    (P := fun x => deps.(_depsCohs2).(_depsCohs).(_deps).(_paintings).2 x)
+    (f := fun x => (deps.(_depsCohs2).(_depsCohs).(_deps).(_restrFrames).2 0 leR_O θ x)).
   rewrite rew_map with
-    (P := fun x => deps.(_depsCohs2).(_depsCohs).(νSet._deps).(_paintings).2 x)
-    (f := fun x => ((deps.(_depsCohs2).(_depsCohs).(νSet._deps).(
-      _restrFrames).2 k leR_refl ε x))).
+    (P := fun x => deps.(_depsCohs2).(_depsCohs).(_deps).(_paintings).2 x)
+    (f := fun x => ((deps.(_depsCohs2).(_depsCohs).(_deps).(
+      _restrFrames).2 i Hi ε x))).
   rewrite 2 rew_compose.
   apply rew_swap with (P := fun x =>
-    deps.(_depsCohs2).(_depsCohs).(νSet._deps).(_paintings).2 x).
+    deps.(_depsCohs2).(_depsCohs).(_deps).(_paintings).2 x).
   rewrite rew_app_rl. now trivial.
   now apply (RestrOfReflCohs deps).(_frames).2.(UIP).
 Defined.
 
-Fixpoint mkIdReflRestrFrames {p k} (deps: DepsReflCohs p k):
-  mkIdReflRestrFrameTypes (NextDepsRefl deps).
+Fixpoint mkIdReflRestrFramesBelow {p k} (deps: DepsReflCohs p k):
+  mkIdReflRestrFrameBelowTypes (mkDepsReflBelow deps).
   destruct p.
-  - simpl. unshelve econstructor. now exact tt. now intros ε [].
-  - set (h := mkIdReflRestrFrames p k.+1 deps.(1)%depsreflcohs).
+  - simpl. unshelve econstructor. now exact tt. now intros i Hi ε [].
+  - set (h := mkIdReflRestrFramesBelow p k.+1 deps.(1)%depsreflcohs).
     unshelve econstructor.
     + now apply h.
-    + intros ε [l c].
+    + intros i Hi ε [l c].
       unshelve eapply eq_existT_curried.
-      * now exact (h.2 ε l).
-      * now exact (mkIdReflRestrLayer deps ε l c h).
+      * now exact (h.2 i.+1 (⇑ Hi) ε l).
+      * now exact (mkIdReflRestrLayerBelow deps i Hi ε l c h).
 Defined.
 
-Definition mkIdReflRestrFrame {p k} (deps: DepsReflCohs p k):
-  mkIdReflRestrFrameType (NextDepsRefl deps) :=
-  (mkIdReflRestrFrames deps).2.
+Definition mkIdReflRestrBelowFrame {p k} (deps: DepsReflCohs p k):
+  mkIdReflRestrFrameBelowType (mkDepsReflBelow deps) :=
+  (mkIdReflRestrFramesBelow deps).2.
 
-Definition HasRefl {p} (deps: DepsReflCohs p 0)
-  (E: mkFrame (NextDepsRestr (CohsOfReflCohs deps)) -> HSet): Type :=
-  forall (d: FramePrev (NextDepsRestr (CohsOfReflCohs deps)))
-    (c: PaintingPrev (NextDepsRestr (CohsOfReflCohs deps)) d),
-  let l ε := (rew <- mkIdReflRestrFrame deps ε d in c) in
-  E (reflFrame (NextDepsRefl deps) d; l).
+Class DepsReflAbove p k := {
+  _depsRefl: DepsReflBelow p k;
+  _extraDeps: DepsRestrExtension p k _depsRefl.(_depsRestr);
+  _reflFramesAbove': mkReflFrameAboveTypes _depsRefl.(_depsRestr);
+}.
 
-Inductive DepsReflCohsExtension p: forall k (deps: DepsReflCohs p k), Type :=
-| TopReflCohDep `{deps: DepsReflCohs p 0}
-  (L: HasRefl deps (mkPaintings (mkExtraDeps (CohsExtOfReflCohs deps))).2):
-  DepsReflCohsExtension p 0 deps
-| AddReflCohDep {k} (deps: DepsReflCohs p.+1 k):
-  DepsReflCohsExtension p.+1 k deps -> DepsReflCohsExtension p k.+1 deps.(1).
+#[local]
+Instance proj1DepsReflAbove {p k}
+  (deps: DepsReflAbove p.+1 k): DepsReflAbove p k.+1 :=
+{|
+  _depsRefl := deps.(_depsRefl).(1)%depsreflbelow;
+  _extraDeps := (deps.(_depsRefl).(_depsRestr); deps.(_extraDeps));
+  _reflFramesAbove' := deps.(_reflFramesAbove').1;
+|}.
 
-Arguments TopReflCohDep {p deps}.
-Arguments AddReflCohDep {p k}.
+Declare Scope depsreflabove_scope.
+Delimit Scope depsreflabove_scope with depsreflabove.
+Bind Scope depsreflabove_scope with DepsReflAbove.
+Notation "x .(1)" := (proj1DepsReflAbove x%depsreflabove)
+  (at level 1, left associativity, format "x .(1)"): depsreflabove_scope.
 
-Declare Scope extra_depsreflcohs_scope.
-Delimit Scope extra_depsreflcohs_scope with extradepsreflcohs.
-Bind Scope extra_depsreflcohs_scope with DepsReflCohsExtension.
-Notation "( x ; y )" := (AddReflCohDep x y)
-  (at level 0, format "( x ; y )"): extra_depsreflcohs_scope.
+Definition AboveOfReflCohs {p k}
+  (depsCohs: DepsReflCohs p k): DepsReflAbove p k :=
+{|
+  _depsRefl := ReflBelowOfReflCohs depsCohs;
+  _extraDeps := RestrExtOfReflCohs depsCohs;
+  _reflFramesAbove' := depsCohs.(_reflFramesAbove);
+|}.
 
+Definition mkReflPaintingAboveType {p k} (deps: DepsReflAbove p.+1 k) :=
+  forall i (Hi: i <= p)
+    (d: FramePrev deps.(_depsRefl).(_depsRestr))
+    (c: PaintingPrev deps.(_depsRefl).(_depsRestr) d),
+  mkPainting deps.(_extraDeps) (deps.(_reflFramesAbove').2 i Hi d c).
 
-Fixpoint mkReflPainting {p k}
+Fixpoint mkReflPaintingAboveTypes {p}:
+  forall {k} (deps: DepsReflAbove p k), Type :=
+  match p with
+  | 0 => fun _ _ => unit
+  | S p =>
+    fun k deps =>
+    { _: mkReflPaintingAboveTypes deps.(1) &T
+      mkReflPaintingAboveType deps }
+  end.
+
+Class CohReflRestrFrameAboveSupTypeBlock {p k} (deps: DepsRestr p k) := {
+  CohReflRestrFrameAboveSupTypesDef: Type;
+  ReflFramesAboveDef: CohReflRestrFrameAboveSupTypesDef -> mkReflFrameAboveTypes deps;
+}.
+
+Definition mkCohReflRestrFrameAboveSupTypesStep {p k} (deps: DepsReflCohs p.+1 k)
+  (prev: CohReflRestrFrameAboveSupTypeBlock (mkDepsRestr (CohsOfReflCohs deps.(1)))): Type :=
+  { Q: prev.(CohReflRestrFrameAboveSupTypesDef) &T
+    forall q r (Hq: q <= p) (Hr: r <= k) (ε: arity)
+      (d: FrameBase (RestrOfReflCohs deps))
+      (c: PaintingBase (RestrOfReflCohs deps) (RestrExtOfReflCohs deps) d),
+    deps.(_reflFramesAbove).2 q Hq _ ((CohsOfReflCohs deps).(_restrPaintings).2 r Hr ε d c) =
+    mkRestrFrame r Hr ε (((prev.(ReflFramesAboveDef) Q).2) q Hq d c) }.
+
+Definition mkReflLayerAbove {p k} (deps: DepsReflCohs p.+1 k)
+  (reflPaintingsAbove: mkReflPaintingAboveTypes (AboveOfReflCohs deps))
+  (prev: CohReflRestrFrameAboveSupTypeBlock (mkDepsRestr (CohsOfReflCohs deps.(1))))
+  (cohFrames: mkCohReflRestrFrameAboveSupTypesStep deps prev)
+  i (Hi: i <= p)
+  (d: FrameBase (RestrOfReflCohs deps))
+  (c: PaintingBase (RestrOfReflCohs deps) (RestrExtOfReflCohs deps) d):
+  mkLayer
+    (paintings := mkPaintings (RestrExtOfReflCohs deps))
+    (mkDepsRestr (CohsOfReflCohs deps)).(_restrFrames)
+    ((prev.(ReflFramesAboveDef) cohFrames.1).2 i Hi d c) :=
+  fun ε =>
+    rew [(mkDepsRestr (CohsOfReflCohs deps)).(_paintings).2]
+      cohFrames.2 i 0 Hi leR_O ε d c in
+  reflPaintingsAbove.2 i Hi _
+    ((CohsOfReflCohs deps).(_restrPaintings).2 0 leR_O ε d c).
+
+Fixpoint mkCohReflRestrFrameAboveSupTypesAndReflFramesAbove {p k}:
+  forall (deps: DepsReflCohs p k)
+    (reflPaintingsAbove: mkReflPaintingAboveTypes (AboveOfReflCohs deps)),
+    CohReflRestrFrameAboveSupTypeBlock (mkDepsRestr (CohsOfReflCohs deps)) :=
+  match p with
+  | 0 => fun deps reflPaintingsAbove =>
+    {|
+      CohReflRestrFrameAboveSupTypesDef := unit;
+      ReflFramesAboveDef _ :=
+        let reflFrameAbove i (Hi: i <= 0)
+          (d: FramePrev (mkDepsRestr (CohsOfReflCohs deps)))
+          (c: PaintingPrev (mkDepsRestr (CohsOfReflCohs deps)) d) :=
+          (mkReflFrameBelow deps 0 leR_O d;
+            fun ε => rew <- mkIdReflRestrBelowFrame deps 0 leR_O ε d in c) in
+        ((tt; reflFrameAbove): mkReflFrameAboveTypes (mkDepsRestr (CohsOfReflCohs deps)))
+    |}
+  | S p => fun deps reflPaintingsAbove =>
+    let prev := mkCohReflRestrFrameAboveSupTypesAndReflFramesAbove deps.(1)
+      reflPaintingsAbove.1 in
+    {|
+      CohReflRestrFrameAboveSupTypesDef := mkCohReflRestrFrameAboveSupTypesStep deps prev;
+      ReflFramesAboveDef Q :=
+        let prevReflFrames := prev.(ReflFramesAboveDef) Q.1 in
+        let reflFrameAbove i (Hi: i <= p.+1)
+          (d: FramePrev (mkDepsRestr (CohsOfReflCohs deps)))
+          (c: PaintingPrev (mkDepsRestr (CohsOfReflCohs deps)) d) :=
+          match i return i <= p.+1 -> mkFrame (mkDepsRestr (CohsOfReflCohs deps)) with
+          | 0 => fun _ =>
+            (mkReflFrameBelow deps 0 leR_O d;
+              fun ε => rew <- mkIdReflRestrBelowFrame deps 0 leR_O ε d in c)
+          | i.+1 => fun Hi =>
+            (prevReflFrames.2 i Hi d.1 (d.2; c);
+              mkReflLayerAbove deps reflPaintingsAbove prev Q i (⇓ Hi) d.1 (d.2; c))
+          end Hi in
+        (prevReflFrames; reflFrameAbove):
+          mkReflFrameAboveTypes (mkDepsRestr (CohsOfReflCohs deps))
+    |}
+  end.
+
+Definition mkCohReflRestrFrameAboveSupTypes {p k}
   (deps: DepsReflCohs p k)
-  (extraDeps: DepsReflCohsExtension p k deps):
-  mkReflPaintingType (NextDepsRefl deps) (mkExtraDeps (CohsExtOfReflCohs deps)).
+  (reflPaintingsAbove: mkReflPaintingAboveTypes (AboveOfReflCohs deps)): Type :=
+  (mkCohReflRestrFrameAboveSupTypesAndReflFramesAbove deps
+    reflPaintingsAbove).(CohReflRestrFrameAboveSupTypesDef).
+
+Class DepsReflCohs2 p k := {
+  _depsReflCohs: DepsReflCohs p k;
+  _reflPaintingsAbove: mkReflPaintingAboveTypes (AboveOfReflCohs _depsReflCohs);
+  _cohReflRestrFramesAboveSup:
+    mkCohReflRestrFrameAboveSupTypes _depsReflCohs _reflPaintingsAbove;
+}.
+
+#[local]
+Instance proj1DepsReflCohs2 {p k} (depsCohs2: DepsReflCohs2 p.+1 k):
+  DepsReflCohs2 p k.+1 :=
+{|
+  _depsReflCohs := depsCohs2.(_depsReflCohs).(1)%depsreflcohs;
+  _reflPaintingsAbove := depsCohs2.(_reflPaintingsAbove).1;
+  _cohReflRestrFramesAboveSup := depsCohs2.(_cohReflRestrFramesAboveSup).1;
+|}.
+
+Declare Scope depsreflcohs2_scope.
+Delimit Scope depsreflcohs2_scope with depsreflcohs2.
+Bind Scope depsreflcohs2_scope with DepsReflCohs2.
+Notation "x .(1)" := (proj1DepsReflCohs2 x%depsreflcohs2)
+  (at level 1, left associativity, format "x .(1)"): depsreflcohs2_scope.
+
+Definition ReflBelowOfReflCohs2 {p k}
+  (depsCohs2: DepsReflCohs2 p k): DepsReflBelow p k :=
+  ReflBelowOfReflCohs depsCohs2.(_depsReflCohs).
+
+Definition RestrOfReflCohs2 {p k}
+  (depsCohs2: DepsReflCohs2 p k): DepsRestr p k :=
+  RestrOfReflCohs depsCohs2.(_depsReflCohs).
+
+Definition CohsOfReflCohs2 {p k}
+  (depsCohs2: DepsReflCohs2 p k): DepsCohs p k :=
+  CohsOfReflCohs depsCohs2.(_depsReflCohs).
+
+Definition Cohs2OfReflCohs2 {p k}
+  (depsCohs2: DepsReflCohs2 p k): DepsCohs2 p k :=
+ depsCohs2.(_depsReflCohs).(_depsCohs2).
+
+Definition RestrExtOfReflCohs2 {p k}
+  (depsCohs2: DepsReflCohs2 p k): DepsRestrExtension p k
+    (RestrOfReflCohs2 depsCohs2) :=
+  RestrExtOfReflCohs depsCohs2.(_depsReflCohs).
+
+Definition CohsExtOfReflCohs2 {p k}
+  (depsCohs2: DepsReflCohs2 p k): DepsCohsExtension p k
+    (CohsOfReflCohs2 depsCohs2) :=
+  CohsExtOfReflCohs depsCohs2.(_depsReflCohs).
+
+Definition mkReflFramesAbove {p k} (deps: DepsReflCohs2 p k):
+  mkReflFrameAboveTypes (mkDepsRestr (CohsOfReflCohs2 deps)) :=
+  (mkCohReflRestrFrameAboveSupTypesAndReflFramesAbove deps.(_depsReflCohs)
+    deps.(_reflPaintingsAbove)).(ReflFramesAboveDef)
+      deps.(_cohReflRestrFramesAboveSup).
+
+Definition mkReflFrameAbove {p k} (deps: DepsReflCohs2 p k):
+  forall i (Hi: i <= p)
+    (d: FramePrev (mkDepsRestr (CohsOfReflCohs2 deps)))
+    (c: PaintingPrev (mkDepsRestr (CohsOfReflCohs2 deps)) d),
+  mkFrame (mkDepsRestr (CohsOfReflCohs2 deps)) :=
+  (mkReflFramesAbove deps).2.
+
+Definition mkDepsReflAbove {p k}
+  (depsCohs2: DepsReflCohs2 p k): DepsReflAbove p.+1 k :=
+{|
+  _depsRefl := mkDepsReflBelow depsCohs2.(_depsReflCohs);
+  _extraDeps := mkExtraDeps (CohsExtOfReflCohs2 depsCohs2);
+  _reflFramesAbove' := mkReflFramesAbove depsCohs2;
+|}.
+
+Definition HasRefl {p} (deps: DepsReflCohs2 p 0)
+  (E: mkFrame (mkDepsRestr (CohsOfReflCohs2 deps)) -> HSet): Type :=
+  forall i (Hi: i <= p)
+    (d: FramePrev (mkDepsRestr (CohsOfReflCohs2 deps)))
+    (c: PaintingPrev (mkDepsRestr (CohsOfReflCohs2 deps)) d),
+  E (mkReflFrameAbove deps i Hi d c).
+
+Inductive DepsReflCohs2Extension p: forall k (deps: DepsReflCohs2 p k), Type :=
+| TopReflCoh2Dep {deps: DepsReflCohs2 p 0}
+  (L: HasRefl deps (mkPaintings (mkExtraDeps (CohsExtOfReflCohs2 deps))).2):
+  DepsReflCohs2Extension p 0 deps
+| AddReflCoh2Dep {k} (deps: DepsReflCohs2 p.+1 k):
+  DepsReflCohs2Extension p.+1 k deps -> DepsReflCohs2Extension p k.+1 deps.(1).
+
+Arguments TopReflCoh2Dep {p deps}.
+Arguments AddReflCoh2Dep {p k}.
+
+Declare Scope extra_depsreflcohs2_scope.
+Delimit Scope extra_depsreflcohs2_scope with extradepsreflcohs2.
+Bind Scope extra_depsreflcohs2_scope with DepsReflCohs2Extension.
+Notation "( x ; y )" := (AddReflCoh2Dep x y)
+  (at level 0, format "( x ; y )"): extra_depsreflcohs2_scope.
+
+Fixpoint mkReflPaintingAbove {p k}
+  (deps: DepsReflCohs2 p k)
+  (extraDeps: DepsReflCohs2Extension p k deps):
+  mkReflPaintingAboveType (mkDepsReflAbove deps).
 Proof.
-  intros d c.
+  intros i Hi d c.
   destruct extraDeps.
-  - unshelve econstructor.
-    + intros ε. now exact (rew <- mkIdReflRestrFrame deps ε d in c).
-    + now exact (L d c).
+  - now exact (L i Hi d c).
   - destruct c as [l c'].
     unshelve econstructor.
-    + apply mkReflLayer.
-      * now exact (deps.(_reflPaintingDeps)).
-      * now exact l.
-    + now exact (mkReflPainting p.+1 k deps extraDeps (d; l) c').
+    + now apply (mkReflLayerAbove _ deps.(_reflPaintingsAbove)).
+    + now exact (mkReflPaintingAbove p.+1 k deps extraDeps i.+1 (⇑ Hi) (d; l) c').
 Defined.
 
-Fixpoint mkReflPaintingsPrefix {p k}:
-  forall (deps: DepsReflCohs p k) (extraDeps: DepsReflCohsExtension p k deps),
-  mkReflPaintingTypes
-    ((NextDepsRefl deps).(1))
-    (NextDepsRestr (CohsOfReflCohs deps);
-    mkExtraDeps (CohsExtOfReflCohs deps)) :=
+Fixpoint mkReflPaintingsAbovePrefix {p k}:
+  forall (deps: DepsReflCohs2 p k) (extraDeps: DepsReflCohs2Extension p k deps),
+  mkReflPaintingAboveTypes ((mkDepsReflAbove deps).(1)) :=
   match p with
   | 0 => fun _ _ => tt
   | S p =>
     fun deps extraDeps =>
-      (mkReflPaintingsPrefix deps.(1) (deps; extraDeps);
-       mkReflPainting deps.(1) (deps; extraDeps))
+      (mkReflPaintingsAbovePrefix deps.(1) (deps; extraDeps);
+       mkReflPaintingAbove deps.(1) (deps; extraDeps))
   end.
 
-Definition mkReflPaintings {p k}:
-  forall (deps: DepsReflCohs p k) (extraDeps: DepsReflCohsExtension p k deps),
-  mkReflPaintingTypes (NextDepsRefl deps)
-    (mkExtraDeps (CohsExtOfReflCohs deps)) :=
+Definition mkReflPaintingsAbove {p k}:
+  forall (deps: DepsReflCohs2 p k) (extraDeps: DepsReflCohs2Extension p k deps),
+  mkReflPaintingAboveTypes (mkDepsReflAbove deps) :=
   fun deps extraDeps =>
-    (mkReflPaintingsPrefix deps extraDeps; mkReflPainting deps extraDeps).
+    (mkReflPaintingsAbovePrefix deps extraDeps; mkReflPaintingAbove deps extraDeps).
 
+Fixpoint mkReflPaintingBelow {p k}
+  (deps: DepsReflCohs2 p k)
+  (extraDeps: DepsReflCohs2Extension p k deps):
+  mkReflPaintingBelowType
+    (mkDepsReflBelow deps.(_depsReflCohs))
+    (mkExtraDeps (CohsExtOfReflCohs2 deps)).
+Proof.
+  intros i Hi d c.
+  destruct i.
+  - unshelve econstructor.
+    + intros ε.
+      rewrite (mkIdReflRestrBelowFrame deps.(_depsReflCohs) 0 leR_O ε d).
+      now exact c.
+    + refine (rew _ in mkReflPaintingAbove deps extraDeps 0 leR_O d c).
+      f_equal.
+      unfold mkDepsReflAbove, mkDepsReflBelow; simpl. 
+      Fail reflexivity.
+      now destruct p.
+  - destruct extraDeps; [now contradiction |].
+    destruct c as [l c'].
+    unshelve econstructor.
+    + now exact (mkReflLayerBelow _ _
+        deps.(_depsReflCohs).(_reflPaintingsBelow) _ _ i Hi d l).
+    + now exact (mkReflPaintingBelow p.+1 k deps extraDeps i (⇓ Hi) (d; l) c').
+Defined.
+
+Fixpoint mkReflPaintingsBelowPrefix {p k}:
+  forall (deps: DepsReflCohs2 p k) (extraDeps: DepsReflCohs2Extension p k deps),
+  mkReflPaintingBelowTypes
+    ((mkDepsReflBelow deps.(_depsReflCohs)).(1))
+    (mkDepsRestr (CohsOfReflCohs2 deps);
+    mkExtraDeps (CohsExtOfReflCohs2 deps)) :=
+  match p with
+  | 0 => fun _ _ => tt
+  | S p =>
+    fun deps extraDeps =>
+      (mkReflPaintingsBelowPrefix deps.(1) (deps; extraDeps);
+       mkReflPaintingBelow deps.(1) (deps; extraDeps))
+  end.
+
+Definition mkReflPaintingsBelow {p k}:
+  forall (deps: DepsReflCohs2 p k) (extraDeps: DepsReflCohs2Extension p k deps),
+  mkReflPaintingBelowTypes
+    (mkDepsReflBelow deps.(_depsReflCohs))
+    (mkExtraDeps (CohsExtOfReflCohs2 deps)) :=
+  fun deps extraDeps =>
+    (mkReflPaintingsBelowPrefix deps extraDeps; mkReflPaintingBelow deps extraDeps).
+
+(*
 Definition mkCohReflRestrPaintingType {p k}
   (deps: DepsReflCohs p.+1 k)
   (extraDeps: DepsReflCohsExtension p.+1 k deps): Type :=
   forall (ε: arity) i (Hi: i <= k)
-    (d: ReflFrameBase (ReflOfReflCohs deps))
-    (c: ReflPaintingBase (ReflOfReflCohs deps) (RestrExtOfReflCohs deps) d),
+    (d: ReflFrameBase (ReflBelowOfReflCohs deps))
+    (c: ReflPaintingBase (ReflBelowOfReflCohs deps) (RestrExtOfReflCohs deps) d),
   rew [ReflPaintingBase
-        (toDepsRefl deps.(_depsCohs2).(_depsCohs) deps.(_reflFrameDeps))
+        (toDepsReflBelow deps.(_depsCohs2).(_depsCohs) deps.(_reflFrameDeps))
         deps.(_depsCohs2).(_depsCohs).(_extraDeps)]
   deps.(_cohReflRestrFrames).2 i Hi ε d in
   deps.(_reflPaintingDeps).2 ((RestrOfReflCohs deps).(_restrFrames).2 i Hi ε d)
     ((CohsOfReflCohs deps).(_restrPaintings).2 i Hi ε d c) =
-  mkRestrPainting (CohsExtOfReflCohs deps.(1)) i (↑ Hi) ε (reflFrame (NextDepsRefl deps.(1)) d)
+  mkRestrPainting (CohsExtOfReflCohs deps.(1)) i (↑ Hi) ε (reflFrame (mkDepsReflBelow deps.(1)) d)
     (mkReflPainting deps.(1) (deps; extraDeps) d c).
 
 Fixpoint mkCohReflRestrPaintingTypes {p}:
@@ -492,25 +715,25 @@ Definition Cohs2OfReflCohs2 {p k}
   (depsCohs2: DepsReflCohs2 p k): DepsCohs2 p k :=
   depsCohs2.(_depsReflCohs).(_depsCohs2).
 
-Definition ReflOfReflCohs2 {p k}
-  `(depsCohs2: DepsReflCohs2 p k): DepsReflRestr p k :=
-  ReflOfReflCohs (depsCohs2.(_depsReflCohs)).
+Definition ReflBelowOfReflCohs2 {p k}
+  (depsCohs2: DepsReflCohs2 p k): DepsReflBelow p k :=
+  ReflBelowOfReflCohs (depsCohs2.(_depsReflCohs)).
 
 Definition RestrOfReflCohs2 {p k}
-  `(depsCohs2: DepsReflCohs2 p k): DepsRestr p k :=
-  (ReflOfReflCohs (depsCohs2.(_depsReflCohs))).(_deps).
+  (depsCohs2: DepsReflCohs2 p k): DepsRestr p k :=
+  (ReflBelowOfReflCohs (depsCohs2.(_depsReflCohs))).(_deps).
 
 Definition CohsOfReflCohs2 {p k}
-  `(depsCohs2: DepsReflCohs2 p k): DepsCohs p k :=
+  (depsCohs2: DepsReflCohs2 p k): DepsCohs p k :=
   depsCohs2.(_depsReflCohs).(_depsCohs2).(_depsCohs).
 
 Definition RestrExtOfReflCohs2 {p k}
-  `(depsCohs2: DepsReflCohs2 p k): DepsRestrExtension p k
+  (depsCohs2: DepsReflCohs2 p k): DepsRestrExtension p k
     (RestrOfReflCohs2 depsCohs2) :=
   depsCohs2.(_depsReflCohs).(_depsCohs2).(_depsCohs).(_extraDeps).
 
 Definition CohsExtOfReflCohs2 {p k}
-  `(depsCohs2: DepsReflCohs2 p k): DepsCohsExtension p k
+  (depsCohs2: DepsReflCohs2 p k): DepsCohsExtension p k
     (CohsOfReflCohs2 depsCohs2) :=
   depsCohs2.(_depsReflCohs).(_depsCohs2).(_extraDepsCohs).
 
@@ -534,10 +757,10 @@ Notation "x .(1)" := (proj1DepsReflCohs2 x%depsreflcohs2)
 Definition mkCohReflRestrLayer {p k}
   (deps: DepsReflCohs2 p.+1 k)
   (ε: arity) i (Hi: i <= k)
-  (d: mkFrame (((toDepsRefl
+  (d: mkFrame (((toDepsReflBelow
     (mkDepsCohs (Cohs2OfReflCohs2 deps))
     (mkReflFrames deps.(_depsReflCohs)))).(_deps).(1).(1)))
-  (l: mkLayer (toDepsRefl
+  (l: mkLayer (toDepsReflBelow
     (mkDepsCohs (Cohs2OfReflCohs2 deps))
     (mkReflFrames deps.(_depsReflCohs))).(_deps).(1).(_restrFrames) d)
   (prevCohReflRestrFrames:
@@ -567,40 +790,40 @@ Proof.
   unfold mkRestrLayer, mkReflLayer.
   rewrite <- map_subst_app, <- !map_subst.
 
-  set (d0 := restrFrame 0 leR_O (toDepsRefl
+  set (d0 := restrFrame 0 leR_O (toDepsReflBelow
     (mkDepsCohs (Cohs2OfReflCohs2 deps).(1))
     (mkReflFrames deps.(_depsReflCohs).(1))).(_deps) θ d).
 
   assert (h :
     (mkDepsCohs (Cohs2OfReflCohs2 deps)).(1).(_restrPaintings).2 i (↑ Hi) ε
-      (reflFrame (toDepsRefl
+      (reflFrame (toDepsReflBelow
         (mkDepsCohs (Cohs2OfReflCohs2 deps).(1))
         (mkReflFrames deps.(_depsReflCohs).(1))) d0)
       ((mkReflPaintings deps.(_depsReflCohs).(1)
         (deps.(_depsReflCohs); deps.(_extraDepsRefl))).2 d0 (l θ)) =
     mkRestrPainting (CohsExtOfReflCohs deps.(_depsReflCohs).(1)) i  (↑ Hi) ε
-      ((NextDepsRefl deps.(_depsReflCohs).(1)).(_reflFrames).2 d0)
+      ((mkDepsReflBelow deps.(_depsReflCohs).(1)).(_reflFrames).2 d0)
       (mkReflPainting deps.(_depsReflCohs).(1)
          (deps.(_depsReflCohs); deps.(_extraDepsRefl)) d0 (l θ)))
   by reflexivity; rewrite h; clear h.
 
   rewrite <- (deps.(_cohReflRestrPaintings).2 ε i Hi d0 (l θ)).
   rewrite rew_map with
-    (P := fun b => (NextDepsRestr (CohsOfReflCohs2 deps).(1)).(_paintings).2 b)
-    (f := fun x => (NextDepsRestr (CohsOfReflCohs2 deps).(1)).(_restrFrames).2
+    (P := fun b => (mkDepsRestr (CohsOfReflCohs2 deps).(1)).(_paintings).2 b)
+    (f := fun x => (mkDepsRestr (CohsOfReflCohs2 deps).(1)).(_restrFrames).2
       0 leR_O θ x).
   rewrite rew_map with
     (P := fun rf => ReflPaintingBase _ _ rf)
-    (f := fun d0 => reflFrame (toDepsRefl _ _) d0).
+    (f := fun d0 => reflFrame (toDepsReflBelow _ _) d0).
   rewrite rew_map with
     (P := fun b => (mkDepsCohs (Cohs2OfReflCohs2 deps)).(1).(
-        νSet._deps).(_paintings).2 b)
+        _deps).(_paintings).2 b)
     (f := fun d0 => (mkDepsCohs (Cohs2OfReflCohs2 deps)).(1).(
-      νSet._deps).(_restrFrames).2 i (↑ Hi) ε d0).
+      _deps).(_restrFrames).2 i (↑ Hi) ε d0).
   rewrite 4 rew_compose.
   apply rew_swap with
     (P := fun b => (mkDepsCohs (Cohs2OfReflCohs2 deps)).(1).(
-      νSet._deps).(_paintings).2 b).
+      _deps).(_paintings).2 b).
   rewrite rew_app_rl. now trivial.
   now apply (mkFrame (RestrOfReflCohs2 deps).(1)).(UIP).
 Defined.
@@ -637,7 +860,7 @@ Proof.
 Defined.
 
 Inductive DepsReflCohs2Extension p: forall k (deps: DepsReflCohs2 p k), Type :=
-| TopReflCohDep2 `{deps: DepsReflCohs2 p 0}
+| TopReflCohDep2 {deps: DepsReflCohs2 p 0}
   (L: HasRefl
     (mkDepsReflCohs deps)
     (mkPaintings (mkExtraDeps (CohsExtOfReflCohs (mkDepsReflCohs deps)))).2):
@@ -673,7 +896,7 @@ Proof.
   intros ε i Hi d [l c].
   destruct i.
   - now trivial.
-  - unfold ReflPaintingBase, PaintingBase, toDepsRefl; simpl.
+  - unfold ReflPaintingBase, PaintingBase, toDepsReflBelow; simpl.
     destruct extraDeps.
     + now contradiction.
     + unshelve eapply (eq_existT_curried_dep
@@ -701,7 +924,7 @@ Definition dgnDepsRestr {p} (C: νSetData p): DepsRestr p 0 :=
   toDepsRestr C.(restrFrames).
 
 Definition dgnDepsRefl {p} (C: νSetData p)
-  (reflFrames: mkReflFrameTypes (dgnDepsRestr C)): DepsReflRestr p 0 :=
+  (reflFrames: mkReflFrameTypes (dgnDepsRestr C)): DepsReflBelow p 0 :=
   {|
     _deps := dgnDepsRestr C;
     _reflFrames := reflFrames;
@@ -933,9 +1156,11 @@ CoInductive νDgnSetFrom n
 }.
 
 Definition νDgnSets (X: νSets) := νDgnSetFrom 0 tt X tt.
+*)
 
 End νDgnSet.
 
+(*
 Module νDgnSetUnit := νDgnSet νSet.ArityUnit.
 Module νDgnSetBool := νDgnSet νSet.ArityBool.
 
@@ -950,3 +1175,4 @@ Example Cubical1 :=
 
 Print Simplicial1.
 Print Cubical1.
+*)
